src/Untyped/Beta.v
@@ -1,0 +1,81 @@
+(* Add LoadPath "~/src/tractatus/src/Untyped/". *)
+
+Require Import String.
+Require Import Coq.Arith.EqNat.
+Require Import Coq.Relations.Relation_Operators.
+
+Require Import Syntax.
+Require Import Substitute.
+
+Module Export Beta.
+(**
+  Beta reduction amounts to taking a term of the form
+  [(lambda x . b) t] and producing [[x:=t]b]. If the term given
+  is not of this form, then return the term. In this manner, it
+  acts like the identity.
+*)
+
+Fixpoint Beta (t:Term) : Term :=
+  match t with
+  | App (Lam body) t' => [(BId 0):=t']body
+  | App t' t'' => match (Beta t') with
+                  | (Lam body) => [(BId 0):=t'']body
+                  | _ as r' => r'
+                  end
+  | _ => t
+  end.
+
+Example i_combinator_is_identity :
+  forall (t : Term),
+  Beta (App Combinator.I t) = t.
+Proof.
+  (* unfold the definitions, then apply Id equality *)
+  intuition.
+  unfold Beta; unfold Combinator.I; unfold subst; apply eq_id.
+Qed.
+
+(** Definition. A term is in Beta Normal Form iff it doesn't have any
+    subterms of the form [App (lambda x. body) R]. *)
+Fixpoint BetaNF (M:Term) : Prop :=
+  match M with
+  | BVar _ => True
+  | FVar _ => True
+  | Lam body => BetaNF body
+  | App (Lam _) _ => False
+  | App M' N => (BetaNF M')/\(BetaNF N)
+  end.
+
+Example Omega_combinator_isnt_beta_nf :
+  ~(BetaNF Combinator.Omega).
+Proof.
+  intros.
+
+  unfold Combinator.Omega; (* Unfold the definitions *)
+  unfold Combinator.omega;
+  unfold BetaNF.
+
+  simpl; tauto. (* And it's obvious. *)
+Qed.
+
+Definition value (t:Term) : Prop := BetaNF t.
+Hint Unfold value.
+Reserved Notation "t1 '⇒' t2" (at level 40).
+
+Inductive step : Term -> Term -> Prop :=
+  | ST_AppAbs : forall t v,
+         value v ->
+         (App (Lam t) v) ⇒ [BId 0:=v]t
+  | ST_App1 : forall t1 t1' t2,
+         t1 ⇒ t1' ->
+         App t1 t2 ⇒ App t1' t2
+  | ST_App2 : forall v1 t2 t2',
+         value v1 ->
+         t2 ⇒ t2' ->
+         App v1 t2 ⇒ App v1 t2'
+where "t1 '⇒' t2" := (step t1 t2).
+Hint Constructors step.
+
+Notation multistep := (clos_refl_trans step).
+Notation "t1 '⇒*' t2" := (multistep t1 t2) (at level 40).
+
+End Beta.
