src/Untyped/Substitute.v
@@ -1,0 +1,217 @@
+(* Add LoadPath "~/src/tractatus/src/Untyped/". *)
+
+Require Import String.
+Require Import Coq.Arith.EqNat.
+Require Import Coq.Relations.Relation_Operators.
+
+Require Import Syntax.
+
+Module Export Substitute.
+(** * Capture-free substitution.
+
+Definition (Barendregt 2.1.15). The result of substituting
+[N] for [x] in [M] (denoted [[x:=N]M]) is defined as follows:
+ - [[x:=N] x = N]
+ - [[x:=N] y = y] (for [y <> x])
+ - [[x:=N] (Lam M) = Lam ([x:=N]M)]
+ - [[x:=N] (App M1 M2) = App ([x:=N]M1) ([x:=N]M2)]
+*)
+Reserved Notation "'[' x ':=' s ']' t" (at level 20).
+
+(* Substitute [s] for [x] in term [t]. *)
+Fixpoint subst (x:Id) (s:Term) (t:Term) : Term :=
+  match t with
+  | FVar x' => if (eq_id_dec (FId x') x) then s else t
+  | BVar n' => if (eq_id_dec (BId n') x) then s else t
+  | Lam b => match x with
+             | FId s' => Lam ([x:=s] b)
+             | BId n => Lam ([(BId (S n)):=s] b)
+             end
+  | App t1 t2 => App ([x:=s] t1) ([x:=s] t2)
+  end
+where "'[' x ':=' s ']' t" := (subst x s t).
+
+
+(** Here are a few "helper functions" with [subst] that should be
+    immediately obvious.
+*)
+Lemma subst_free_var :
+  forall (x:string) (N:Term),
+  [FId x := N]FVar x = N.
+Proof.
+  intros.
+  unfold subst. apply eq_id.
+Qed.
+
+Lemma subst_free_var_denied :
+  forall (x y:string) (L:Term),
+  x<>y -> ([FId y := L]FVar x)=FVar x.
+Proof.
+  intros.
+  unfold subst.
+  apply neq_id. (* But [FId x <> FId y] *)
+  contradict H. (* If it did... *)
+  inversion H.
+  reflexivity.
+Qed.
+
+Lemma subst_bvar_denied :
+  forall (x:string) (n:nat) (L:Term),
+  [FId x:=L]BVar n = BVar n.
+Proof.
+  intros.
+  unfold subst. (* By definition of [subst], we see *)
+  apply neq_id. (* [BId n <> FId x] *)
+  discriminate. (* by looking at it! *)
+Qed.
+Lemma unfold_one_step :
+  forall (x y:string) (L N:Term),
+  x<>y->~(Id_in_FV (FId x) L)->[FId x := [FId y := L]N]FVar x = [FId y:=L]N.
+Proof.
+  intros.
+  unfold subst.
+  apply eq_id.
+Qed.
+
+Lemma identity_subst :
+  forall (y:string) (L:Term),
+  [FId y := L]FVar y = L.
+Proof.
+  intuition.
+  unfold subst; rewrite eq_id; reflexivity.
+Qed.
+Lemma subst_lambda_swap :
+  forall (x:string) (M N:Term),
+  [FId x:=N]Lam M=Lam([FId x:=N]M).
+Proof.
+  intuition.
+Qed.
+Lemma subst_app_functoriality :
+  forall (x:string) (M1 M2 N:Term),
+  [FId x:=N]App M1 M2=App ([FId x:=N]M1) ([FId x:=N]M2).
+Proof.
+  intuition.
+Qed.
+
+Lemma absent_id_doesnt_subst :
+  forall (s:string) (M N:Term),
+  ~(Id_in_FV (FId s) M) -> [(FId s):=N]M = M.
+Proof.
+  intros.
+  induction M.
+  (* Case: M = FVar s0 *)
+    rewrite subst_free_var_denied. reflexivity. apply trivial_FV_notin_FV in H. trivial.
+  (* Case: M = BVar s0 *)
+    unfold subst. apply neq_id. discriminate.
+  (* Case: M = Lam M' *)
+    rewrite subst_lambda_swap. rewrite IHM. reflexivity. auto.
+  (* Case: M = App M1 M2 *)
+    rewrite subst_app_functoriality. rewrite IHM1. rewrite IHM2. reflexivity.
+    rewrite <- app_FV_denied_l in H; auto. rewrite <- app_FV_denied_l in H; auto.
+Qed.
+
+(** ** Non-Commutativity of Substitution
+
+  The big property everyone wants to prove about substitution is
+  that it's not commutative. That is to say, if we first substitute
+  [x:=t1], then substitute [y:=t2], it's not the same as going the
+  other way around. Why?
+  
+  What if [t1] has [y] in it? In order to swap the order of substitutions,
+  we need to address this issue by having [y:=t2] be followed by
+  [x:=[y:=t2]t1].
+  
+  Mathematicians have given this statement the imaginative name of...
+*)
+
+Lemma substitution_lemma_subcase_11 :
+  forall (x y:string) (L M N:Term),
+  x<>y /\ ~(Id_in_FV (FId x) L) ->
+  [(FId y):=L]([(FId x):=N] (FVar x)) = [(FId x):=([(FId y):=L] N)]([(FId y):=L] (FVar x)).
+Proof.
+  intuition.
+  rewrite subst_free_var; rewrite subst_free_var_denied.
+  rewrite unfold_one_step. reflexivity. auto. auto. auto.
+Qed.
+
+Lemma substitution_lemma_subcase_12 :
+  forall (x y:string) (L M N:Term),
+  x<>y /\ ~(Id_in_FV (FId x) L) ->
+  [(FId y):=L]([(FId x):=N] (FVar y)) = [(FId x):=([(FId y):=L] N)]([(FId y):=L] (FVar y)).
+Proof.
+  intros.
+  rewrite subst_free_var; rewrite subst_free_var_denied.
+  rewrite identity_subst. rewrite absent_id_doesnt_subst. reflexivity.
+  inversion H. assumption. inversion H. auto.
+Qed.
+
+Lemma substitution_lemma_subcase_13 :
+  forall (x y s:string) (L M N:Term),
+  x<>y -> x<>s -> y<>s -> ~(Id_in_FV (FId x) L) ->
+  [FId y := L]([FId x := N]FVar s) = [FId x := [FId y := L]N]([FId y := L]FVar s).
+Proof.
+  intros.
+  repeat (rewrite subst_free_var_denied). (* There's nothing to substitute *)
+  reflexivity. auto. auto. auto. (* so we're done *)
+Qed.
+
+(* Barendregt 2.1.16 *)
+Theorem substitution_lemma : (* I didn't name it... *)
+  forall (x y:string) (L M N:Term),
+  x<>y -> ~(Id_in_FV (FId x) L) ->
+  [(FId y):=L]([(FId x):=N] M) = [(FId x):=([(FId y):=L] N)]([(FId y):=L] M).
+Proof.
+  intros.
+  induction M.
+  (* Case: M = FVar s *)
+    case (string_dec s x).
+    (* Subcase: s = x *)
+    - intuition.
+      rewrite e. (* plugin our assumption [s = x] *) 
+      apply substitution_lemma_subcase_11. auto. auto. (* and it follows from our lemma *)
+    (* Subcase: s = y *)
+    - case (string_dec s y).
+      intros.
+      rewrite e.
+      apply substitution_lemma_subcase_12. auto. auto.
+    (* Subcase: s <> x and s <> y *)
+      intuition. apply substitution_lemma_subcase_13. auto. auto. auto. auto. auto.
+  (* Case: M = BVar s *)
+  - repeat (rewrite subst_bvar_denied). (* We cann't substitute [FId] for a [BVar] *)
+    reflexivity. (* So we get [BVar n = BVar n], by reflexivity. *)
+  (* Case: M = Lam body *)
+  - repeat (rewrite subst_lambda_swap). (* We see this is true if it's true 
+                                           for the body of the lambda 
+                                           expressions. *)
+    rewrite IHM; reflexivity. (* Then by inductive hypothesis, it's true. *)
+  (* Case: M = App M1 M2 *)
+  - repeat (rewrite subst_app_functoriality).
+    rewrite IHM1; rewrite IHM2; reflexivity. (* Then by inductive hypothesis, it's true. *)
+Qed.
+
+(** Barendregt 2.1.17.i *)
+Proposition subst_apply_rand :
+  forall (M M' N:Term) (x:Id),
+  M=M' -> [x:=N]M = [x:=N]M'.
+Proof.
+  intros. rewrite H. reflexivity.
+Qed.
+
+(** Barendregt 2.1.17.ii *)
+Proposition subst_apply_rator :
+  forall (M N N':Term) (x:Id),
+  N=N' -> [x:=N]M = [x:=N']M.
+Proof.
+  intros. rewrite H. reflexivity.
+Qed.
+
+(** Barendregt 2.1.17.iii *)
+Proposition subst_apply_rand_rator :
+  forall (M M' N N':Term) (x:Id),
+  M=M' -> N=N' -> [x:=N]M = [x:=N']M'.
+Proof.
+  intros.
+  rewrite H. rewrite H0. reflexivity.
+Qed.
+
+End Substitute.
